cedar-lean/Cedar/Thm/Lemmas/TypecheckerInversion.lean
@@ -1,0 +1,54 @@
+/-
+ Copyright 2022-2023 Amazon.com, Inc. or its affiliates. All Rights Reserved.
+
+ Licensed under the Apache License, Version 2.0 (the "License");
+ you may not use this file except in compliance with the License.
+ You may obtain a copy of the License at
+
+      https://www.apache.org/licenses/LICENSE-2.0
+
+ Unless required by applicable law or agreed to in writing, software
+ distributed under the License is distributed on an "AS IS" BASIS,
+ WITHOUT WARRANTIES OR CONDITIONS OF ANY KIND, either express or implied.
+ See the License for the specific language governing permissions and
+ limitations under the License.
+-/
+
+import Cedar.Spec
+import Cedar.Thm.Lemmas.Std
+import Cedar.Thm.Lemmas.Types
+import Cedar.Validation
+
+/-!
+This file contains type checker inversion lemmas.
+-/
+
+namespace Cedar.Thm
+
+open Cedar.Data
+open Cedar.Spec
+open Cedar.Validation
+
+
+theorem type_of_not_inversion {x₁ : Expr} {c₁ c₂ : Capabilities} {env : Environment} {ty : CedarType}
+  (h₁ : typeOf (Expr.unaryApp .not x₁) c₁ env = Except.ok (ty, c₂)) :
+  c₂ = ∅ ∧
+  ∃ bty c₁',
+    ty = .bool bty.not ∧
+    typeOf x₁ c₁ env = Except.ok (.bool bty, c₁')
+:= by
+  simp [typeOf] at h₁
+  cases h₂ : typeOf x₁ c₁ env <;> simp [h₂] at h₁
+  case ok res =>
+    rcases res with ⟨ty₁, c₁'⟩
+    simp [typeOfUnaryApp] at h₁
+    split at h₁ <;> try contradiction
+    case mk.h_1 _ ty₁ bty _ =>
+      simp [ok] at h₁
+      apply And.intro
+      case left => simp [h₁]
+      case right =>
+        exists bty, c₁'
+        simp only [and_true, h₁]
+
+end Cedar.Thm
