cedar-lean/Cedar/Thm/Lemmas/Types.lean
@@ -1,0 +1,242 @@
+/-
+ Copyright 2022-2023 Amazon.com, Inc. or its affiliates. All Rights Reserved.
+
+ Licensed under the Apache License, Version 2.0 (the "License");
+ you may not use this file except in compliance with the License.
+ You may obtain a copy of the License at
+
+      https://www.apache.org/licenses/LICENSE-2.0
+
+ Unless required by applicable law or agreed to in writing, software
+ distributed under the License is distributed on an "AS IS" BASIS,
+ WITHOUT WARRANTIES OR CONDITIONS OF ANY KIND, either express or implied.
+ See the License for the specific language governing permissions and
+ limitations under the License.
+-/
+
+import Cedar.Spec
+import Cedar.Thm.Lemmas.Std
+import Cedar.Validation
+
+/-!
+This file contains useful definitions and lemmas about Cedar types.
+
+todo: fill in `sorry`s.
+-/
+
+namespace Cedar.Thm
+
+open Cedar.Data
+open Cedar.Spec
+open Cedar.Validation
+
+----- Definitions -----
+
+def InstanceOfBoolType : Bool → BoolType → Prop
+  | true,  .tt      => True
+  | false, .ff      => True
+  | _,     .anyBool => True
+  | _, _            => False
+
+def InstanceOfEntityType (e : EntityUID) (ety: EntityType) : Prop :=
+  ety = e.ty
+
+def InstanceOfExtType : Ext → ExtType → Prop
+  | .decimal _, .decimal => True
+  | .ipaddr _,  .ipAddr  => True
+  | _, _                 => False
+
+inductive InstanceOfType : Value → CedarType → Prop :=
+  | instance_of_bool (b : Bool) (bty : BoolType)
+      (h₁ : InstanceOfBoolType b bty) :
+      InstanceOfType (.prim (.bool b)) (.bool bty)
+  | instance_of_int :
+      InstanceOfType (.prim (.int _)) .int
+  | instance_of_string :
+      InstanceOfType (.prim (.string _)) .string
+  | instance_of_entity (e : EntityUID) (ety: EntityType)
+      (h₁ : InstanceOfEntityType e ety) :
+      InstanceOfType (.prim (.entityUID e)) (.entity ety)
+  | instance_of_set (s : Set Value) (ty : CedarType)
+      (h₁ : forall v, v ∈ s → InstanceOfType v ty) :
+      InstanceOfType (.set s) (.set ty)
+  | instance_of_record (r : Map Attr Value) (rty : RecordType)
+      -- if an attribute is present, then it has the expected type
+      (h₁ : ∀ (k : Attr) (v : Value) (qty : QualifiedType),
+        rty.find? k = some qty → r.find? k = some v → InstanceOfType v qty.getType)
+      -- required attributes are present
+      (h₂ : ∀ (k : Attr) (qty : QualifiedType), rty.find? k = some qty → qty.isRequired → r.contains k) :
+      InstanceOfType (.record r) (.record rty)
+  | instance_of_ext (x : Ext) (xty : ExtType)
+      (h₁ : InstanceOfExtType x xty) :
+      InstanceOfType (.ext x) (.ext xty)
+
+def InstanceOfRequestType (request : Request) (reqty : RequestType) : Prop :=
+  InstanceOfEntityType request.principal reqty.principal ∧
+  request.action = reqty.action ∧
+  InstanceOfEntityType request.resource reqty.resource ∧
+  InstanceOfType request.context (.record reqty.context)
+
+/--
+For every entity in the store,
+1. The entity's type is defined in the type store.
+2. The entity's attributes match the attribute types indicated in the type store.
+3. The entity's ancestors' types are consistent with the ancestor information
+   in the type store.
+-/
+def InstanceOfEntityTypeStore (entities : Entities) (ets: EntityTypeStore) : Prop :=
+  ∀ uid data, entities.find? uid = some data →
+    ∃ attrTys ancestorTys, ets.find? uid.ty = some (attrTys, ancestorTys) ∧
+      InstanceOfType data.attrs (.record attrTys) ∧
+      ∀ ancestor, ancestor ∈ data.ancestors → ancestor.ty ∈ ancestorTys
+
+/--
+For every action in the entity store, the action's ancestors are consistent
+with the ancestor information in the action store.
+-/
+def InstanceOfActionStore (entities : Entities) (as: ActionStore) : Prop :=
+  ∀ uid data, entities.find? uid = some data → as.contains uid →
+    ∃ ancestors, as.find? uid = some ancestors →
+      ∀ ancestor, ancestor ∈ data.ancestors → ancestor ∈ ancestors
+
+def RequestAndEntitiesMatchEnvironment (env : Environment) (request : Request) (entities : Entities) : Prop :=
+  InstanceOfRequestType request env.reqty ∧
+  InstanceOfEntityTypeStore entities env.ets ∧
+  InstanceOfActionStore entities env.acts
+
+----- Theorems -----
+
+theorem false_is_instance_of_ff :
+  InstanceOfType (Value.prim (Prim.bool false)) (CedarType.bool BoolType.ff)
+:= by
+  apply InstanceOfType.instance_of_bool
+  simp [InstanceOfBoolType]
+
+theorem true_is_instance_of_tt :
+  InstanceOfType (Value.prim (Prim.bool true)) (CedarType.bool BoolType.tt)
+:= by
+  apply InstanceOfType.instance_of_bool
+  simp [InstanceOfBoolType]
+
+theorem bool_is_instance_of_anyBool (b : Bool) :
+  InstanceOfType (Value.prim (Prim.bool b)) (CedarType.bool BoolType.anyBool)
+:= by
+  apply InstanceOfType.instance_of_bool
+  simp [InstanceOfBoolType]
+
+theorem instance_of_ff_is_false {v₁ : Value} :
+  InstanceOfType v₁ (CedarType.bool BoolType.ff) →
+  v₁ = .prim (.bool false)
+:= by
+  intro h₁
+  cases h₁ with
+  | instance_of_bool b _ h₁ =>
+    simp [InstanceOfBoolType] at h₁
+    cases b <;> simp at h₁
+    rfl
+
+theorem instance_of_tt_is_true {v₁ : Value} :
+  InstanceOfType v₁ (CedarType.bool BoolType.tt) →
+  v₁ = .prim (.bool true)
+:= by
+  intro h₁
+  cases h₁ with
+  | instance_of_bool b _ h₁ =>
+    simp [InstanceOfBoolType] at h₁
+    cases b <;> simp at h₁
+    rfl
+
+theorem instance_of_anyBool_is_bool {v₁ : Value} :
+  InstanceOfType v₁ (CedarType.bool BoolType.anyBool) →
+  ∃ b, v₁ = .prim (.bool b)
+:= by
+  intro h₁
+  cases h₁ with
+  | instance_of_bool b _ h₁ =>
+    apply Exists.intro b
+    rfl
+
+theorem instance_of_type_bool_is_bool (v : Value) (ty : CedarType) :
+  InstanceOfType v ty →
+  ty ⊑ .bool .anyBool →
+  ∃ b, v = .prim (.bool b)
+:= by
+  intro h₀ h₁
+  cases v <;> cases ty <;> try cases h₀ <;>
+  try simp [subty, lub?] at h₁
+  case instance_of_bool b bty =>
+    exists b
+
+theorem bool_type_is_inhabited (bty : BoolType) :
+  ∃ b, InstanceOfBoolType b bty
+:= by
+  simp [InstanceOfBoolType]
+  cases bty
+  case tt => apply Exists.intro true; simp only
+  all_goals {
+    apply Exists.intro false; simp only
+  }
+
+theorem entity_type_is_inhabited (ety : EntityType) :
+  ∃ euid, InstanceOfEntityType euid ety
+:= by
+  simp [InstanceOfEntityType]
+  apply Exists.intro (EntityUID.mk ety default)
+  simp only
+
+theorem ext_type_is_inhabited (xty : ExtType) :
+  ∃ x, InstanceOfExtType x xty
+:= by
+  simp [InstanceOfExtType]
+  cases xty
+  case ipAddr =>
+    apply Exists.intro (Ext.ipaddr (default : IPAddr))
+    simp only
+  case decimal =>
+    apply Exists.intro (Ext.decimal (default : Ext.Decimal))
+    simp only
+
+mutual
+theorem type_is_inhabited (ty : CedarType) :
+  ∃ v, InstanceOfType v ty
+:= by
+  match ty with
+  | .bool bty =>
+    rcases (bool_type_is_inhabited bty) with ⟨b, h₁⟩
+    apply Exists.intro (.prim (.bool b))
+    apply InstanceOfType.instance_of_bool _ _ h₁
+  | .int =>
+    apply Exists.intro (.prim (.int default))
+    apply InstanceOfType.instance_of_int
+  | .string =>
+    apply Exists.intro (.prim (.string default))
+    apply InstanceOfType.instance_of_string
+  | .entity ety =>
+    rcases (entity_type_is_inhabited ety) with ⟨euid, h₁⟩
+    apply Exists.intro (.prim (.entityUID euid))
+    apply InstanceOfType.instance_of_entity _ _ h₁
+  | .set ty₁ =>
+    apply Exists.intro (.set Set.empty)
+    apply InstanceOfType.instance_of_set
+    intro v₁ h₁
+    rcases (Set.in_set_means_list_non_empty v₁ Set.empty h₁) with h₂
+    simp [Set.empty] at h₂
+  | .ext xty =>
+    rcases (ext_type_is_inhabited xty) with ⟨x, h₁⟩
+    apply Exists.intro (.ext x)
+    apply InstanceOfType.instance_of_ext _ _ h₁
+  | .record rty =>
+    rcases (record_type_is_inhabited rty) with ⟨r, h₁, h₂⟩
+    apply Exists.intro (.record r)
+    apply InstanceOfType.instance_of_record _ _ h₁ h₂
+
+theorem record_type_is_inhabited (rty : RecordType) :
+  ∃ (r : Map Attr Value),
+    (∀ (k : Attr) (v : Value) (qty : QualifiedType),
+      rty.find? k = some qty → r.find? k = some v → InstanceOfType v qty.getType) ∧
+    (∀ (k : Attr) (qty : QualifiedType), rty.find? k = some qty → qty.isRequired → r.contains k)
+:= by sorry
+
+end
+
+end Cedar.Thm
